auto_generated/hol-kananaskis-10/elf_headerTheory.sml
@@ -14,14 +14,14 @@ struct
   in end;
   val _ = Theory.link_parents
           ("elf_header",
-          Arbnum.fromString "1445345935",
-          Arbnum.fromString "766165")
+          Arbnum.fromString "1445438753",
+          Arbnum.fromString "972064")
           [("lem_set",
            Arbnum.fromString "1445005525",
            Arbnum.fromString "352564"),
            ("elf_types_native_uint",
-           Arbnum.fromString "1445345916",
-           Arbnum.fromString "991129"),
+           Arbnum.fromString "1445438741",
+           Arbnum.fromString "175496"),
            ("default_printing",
            Arbnum.fromString "1445345889",
            Arbnum.fromString "988195")];
